
::: {.theorem  name="Simple Approximation Theorem"}

Give a function: 
$$ d_n(r)=\sum_{k=1}^{n2^{n}} \frac{k-1}{2^{n}} 1_{[\frac{k-1}{2^{n}},\frac{k}{2^{n}})}(r)+n 1_{[n,\infty]}(r), \qquad r\in \overline{\R}_+ $$
Notice that $d_n(r)$ is an increasing right-continuous simple function and  $d_n(r)\nearrow r$ as $n\to \infty$.  

A positive function $f$ on  $E$ is $\mathcal{E}$-measurable iff it is the limit of an increasing sequence of positive simple functions.

:::


::: {.proof}

When a $\limsup$ and a $\liminf$ exists for a simple function sequence, then $\lim f_n$ exists and as for  $n\in \N_+$, $f_n$ is $\mathcal{E}$-measurable, $\lim f_n$ is $\mathcal{E}$-measurable.  
For the converse, let $f_n=d_n\circ f$ is. Then  $f_n \nearrow f$ and $f_n$ is a simple function.

:::


::: {.definition  name="Integrations"}

- $\int fd\mu$ is called the integrations of $f$ according to measure $\mu$, usually noted as $\mu f$.
- $\int_A fd\mu$ is called the integrations of $f$ according to $\mu$ on $\mathcal{E}$-measurable set $A$, noted as $\mu(f 1_A)$.

:::

::: {.theorem  name="Monotone Convergence Theorem"}

Let $(f_n)$ be an increasing sequence in $\mathcal{E}_+$, then: 
$$ \mu(\lim f_n)=\lim \mu f_n $$


:::

::: {.proof}

Let $f_n \nearrow f$, then $\mu f\ge \mu f_n$ for each $n$, so $\mu f \ge \lim \mu f_n$.  
Now need to prove that $\lim \mu f_n\ge \mu f$.  
Fix $b\in \R_+$ and $B\in \mathcal{E}$, where $f$ is $\mathcal{E}$-measurable. Then $\{f_n>b\}\nearrow \{f>b\}$, where let $B_n=B\cap \{f_n>b\}$, then $B_n \nearrow B$, so 
$$ \lim  \mu(B_n)=\mu(B)  $$
and: 
$$ f_n 1_B\ge f_n 1_{B_n}\ge b 1_{B_n} $$
then 
$$ \mu(f_n 1_B)\ge \mu(b 1_{B_n})=b\mu(1_{B_n}) $$
Take limits for each side: 
$$ \lim  \mu(f_n 1_B)\ge b\mu(B) $$
Let $g$ be a positive simple function s.t. $f\ge g$ holds on $E$. Let $g=\sum_{i=1}^{m} b_i 1_{B_i}$ where on each $B_i$, $f\ge b_i$ holds. Then: 
$$ \lim  \mu(f_n 1_{B_i})\ge b_i\mu(B_i)\qquad i=1,2,\ldots,m $$
Let $g$ has the canonical representation, then 
$$ \lim_n \mu f_n=\lim_n \sum_{i=1}^{m} \mu(f_n 1_{B_i})=\sum_{i=1}^{m} \lim_n \mu(f_n 1_{B_i})\ge \mu g $$
Let $g=d_k\circ f$ and change $g$ to its canonical representation, then  
$$ \lim_n \mu f_n \ge \mu(d_k\circ f) $$
holds for every $k$, then let $k\to \infty$, we get $\lim  \mu f_n\ge \mu f$.
Now we prove the theorem.

:::


::: {.theorem  name="Fatou's Lamma"}

Let $(f_n)\in \mathcal{E_+}$, then 
$$ \mu(\liminf f_n)\le \liminf \mu f_n $$

:::

::: {.proof}

Let $g_m=\inf_{n\ge m}f_n$, notice that $g_m$ is increasing and $g_m \nearrow \liminf f_n$ as $m\to \infty$. By the monotone converge theorem: 
$$ \mu(\liminf f_n)=\lim  \mu g_m $$
Notice that $g_m\le f_n$ for all $n\ge m$, and $\mu g_m\le \mu f_n$ for all $n\ge m$, so $\mu g_m \le \inf_{n\ge m}\mu f_n$, take limit of $m$, 
$$ \lim \mu g_m \le \liminf \mu f_n$$


:::

::: {.theorem  name="Almost Everywhere Theorem"}

Let $(f_n)$ be a sequence of numerical functions on $E$. Suppose that for each $n$, there is $g_n\in \mathcal{E}$ s.t. $f_n=g_n$ a.e. Further suppose for each $n$ that $f_n\ge 0$ a.e. and $f_n\le f_{n+1}$ a.e. Then, $\lim f_n$ exists a.e. is positive a.e. and $\mu(\lim f_n)=\lim \mu f_n$.

:::

::: {.proof}

Let  
$$ N=\bigcup_{n=1} ^{\infty}(L_n\cup M_n\cup N_n) $$
where $L$ denotes the $f_n\le f_{n+1}$ 's zero-measure set, and $N$ denote the $f_n=g_n$ 's and $M$ denotes $f_n\ge 0$ 's.  
For every $x\in E-N$, we have 
$$ 0\le f_1(x)=g_1(x)\le f_2(x)=g_2(x)\ldots $$
so $\lim f_n=\lim g_n$ exists on $E-N$. Then define: 
$$ f(x)=\begin{cases}
	\lim f_n(x) & x\notin N \\
	0 & x\in N
\end{cases} $$
Then $(g_n 1_{E-N})\nearrow f$ on $E$. So 
$$ \mu f=\lim \mu(g_n 1_{E-N})=\lim \mu g_n $$


:::

::: {.theorem  name="Integral characterization theorem"}

Let $(E,\mathcal{E})$ be a measurable space. Let $L$ be a mapping from $\mathcal{E_+}$ into $\overline{\R}_+$ then there is a unique measure $\mu$ on $(E,\mathcal{E})$ s.t. $L(f)=\mu f$ for every $f\in \mathcal{E_+}$ iff:
-  $f=0\implies L(f)=0$ 
- $f,g\in \mathcal{E_+}$ and $a,b\in \R_+\implies L(af+bg)=aL(f)+bL(g)$
- $(f_n)\subset \mathcal{E_+}$ and $f_n \nearrow f\implies L(f_n)\nearrow L(f)$

:::

::: {.proof}

Let there is a function $L$ satisfies above conditions and give a $\mu$ and let $\mu (A)=L(1_A)$, then use those conditions we can prove that $\mu$ is a measure a $(E,\mathcal{E})$.

:::

::: {.definition  name="Image measure"}

let $(F,\mathcal{F})$ and $(E,\mathcal{E})$ be measurable spaces. Let $\nu$ be a measure on $(F,\mathcal{F})$ and let $h:F\to E$ be measurable relative to $\mathcal{F}$ and $\mathcal{E}$, then define a mapping $\nu\circ h^{-1}(B)=\nu(h^{-1}B),\ B\in \mathcal{E}$.  
Then $\nu\circ h^{-1}$ is a measure on $(E,\mathcal{E})$, which is called the image of $\nu$ under $h$.

:::

::: {.theorem  name=""}

For every $f\in \mathcal{E_+}$, we have $(\nu\circ h^{-1})f=\nu(f\circ h)$.

:::

::: {.proof}

Let $L:\mathcal{E}_+\to \overline{\R}_+$ by letting $L(f)=\nu(f\circ h)$. Then as the property of $\nu(f\circ h)$, $f$ satisfies the properties of integral characterization theorem. Then, $L(f)=\mu f$ for some unique measure $\mu$ on $(E,\mathcal{E})$. And 
$$ \mu (B)=L(1_B)=\nu(1_B \circ h)=\nu(h^{-1}B), \qquad B\in \mathcal{E} $$


:::

::: {.definition  name="Standard measurable space"}

Let $(E,\mathcal{E})$ and $(F,\mathcal{F})$ be measurable spaces let $f$ be a bijection from $E$ onto $F$, then  $f$ is called an isomorphism of $(E,\mathcal{E})$ and $(F,\mathcal{F})$ iff $f$ is $\mathcal{E}$-measurable and $f^{-1}$ is $\mathcal{F}$-measurable.  
A measurable space $(E,\mathcal{E})$ is said to be a standard measurable space if it is isomorphic to $(F,\mathcal{B}_F)$ for some Borel set $F$ of $\R$.

:::

::: {.definition  name=""}

Let $\mu$ be a measure on $(E,\mathcal{E})$. It is said to be finite if $\mu (E)\lt \infty$, then $\mu (A)\lt\infty$ for every $A\subset E$.  
It is called a probability measure if $\mu (E)=1$.  
It is said to be $\sigma$-finite if there exists a measurable partition $(E_n)$ of $E$ s.t. for each $n$, $\mu (E_n)\lt \infty$.  
It is said to be $\Sigma$-finite if there exists a sequence of finite measures $(\mu_n)$ s.t. $\mu =\sum_{n}^{} \mu_n$.

:::

::: {.theorem  name=""}

If a measure is $\sigma$-finite then it must be  $\Sigma$-finite.

:::

::: {.proof}

Assume that there is a measure $\mu$ on $(E,\mathcal{E})$ is $\sigma$-finite, where there is a $(E_n)\subset \mathcal{E}$ s.t. $\bigcup_{n} E_n=E$. Then give $(\mu_n)$ s.t. for each $n$, 
$$ \begin{cases}
	\mu_n(E_n)=\mu(E_n) \\
	\mu_n(E-E_n)=0
\end{cases} $$
then $\mu_n(E)=\mu_n(E_n)=\mu (E_n)$, so a $\sigma$-finite measure $\mu$ is a $\Sigma$-fnite measure.

:::

Let $(E,\mathcal{E},\mu)$ be a measure space. Let $p$ be a positive $\mathcal{E}$-measurable function. Define: 
$$ \nu(A)=\mu (p 1_A)=\int_A \mu (dx)p(x),\qquad A\in \mathcal{E}$$


::: {.theorem  name=""}

$\nu$ is a measure on $(E,\mathcal{E})$.

:::

::: {.proof}

- Let  $A,B$ be disjoint sets in $E$, then $\mu (p 1_A)+\mu (p 1_B)=\mu (p 1_{A\cup B})$  
- $\mu (p 1_\varnothing)=0$

:::

::: {.theorem  name=""}

Fix a $p \in \mathcal{E_+}$, and give a measure $\mu$ on $(E,\mathcal{E})$, then there must be a measure $\nu$ satisfying $\nu f=\mu (pf)$ for every $f\in \mathcal{E_+}$.

:::

::: {.proof}

Let $L(f)=\mu (pf)$. Check $L$ :
- $f=0\implies L(f)=0$ 
- Give $f,g\in \mathcal{E_+}$ and $a,b\in \mathbb{R}_+\implies L(af+bg)=\mu (p(af+bg))$ and based on the arithmetic rules on $\mathbb{R}$ and the linearity of $\mu$, $L(af+bg)=aL(f)+bL(g)$ 
- Give $(f_n)\subset \mathcal{E_+}$ and $f_n \nearrow f$, $L(f_n)=\mu (pf_n)$ and as $f_n \nearrow f$, $pf_n \nearrow pf$ so $\lim L(f_n)=\lim \mu (pf_n)$. According to the monotone converging theorem, $\lim \mu (pf_n)=\mu (pf)=L(f)$ 

So there exists a $\nu$ satisfying $\nu f=L(f)=\mu (pf)$.

:::

Written above result in an explicit notation: 
$$ 
\int_E \nu(dx)f(x)=\int_E \mu (dx)p(x)f(x)
$$
then we can change the $\nu(dx)$ with $\mu (dx)p(x)$ where $x\in E$, $p\in \mathcal{E_+}$.


::: {.definition  name="absolutely continuous"}

Let $\nu$ and $\mu$ be measures on a measurable space  $(E,\mathcal{E})$. Then $\nu$ is said to be absolutely continuous respect to $\mu$ if for any set $A\in \mathcal{E}$, $\mu (A)=0\implies\nu(A)=0$.

:::

::: {.theorem  name=""}

If $\nu$ satisfies the conditions $\nu f=\mu(pf)$ for every $f\in \mathcal{E_+}$, then $\nu$ is absolutely continuous with respect to $\mu$.

:::
 

::: {.proof}


Let $\mu (A)=0$, then we need to prove that  $\mu (p \bm{\mathbf{1}}_{A})=0$: 
- Let $p$ is a simple function with a cononical form on $E$ with $p=\sum_{i=1}^{n} a_i \bm{\mathbf{1}}_{B_i}$ and as $(B_i)$ is a partition, $(B_i\cap A)$ is a partition of $A$, noted as $(A_i)$. Then 
$$ 
\mu (p \bm{\mathbf{1}}_{A})=\int_A pd\mu =\sum_{i=1}^{n} a_i \mu (A_i)
$$ 
As $\mu (A)=0$ and $A=\bigcup_{i=1} ^{n}A_i$, $\mu (A)=\sum_{i=1}^{n} \mu (A_i)$, so $\mu (A_i)=0$ for every $i$. So $\mu (p \bm{\mathbf{1}}_{A})=0$.
- Let $p\in \mathcal{E_+}$, give $(p_n)$ s.t. $p_n \nearrow p$ where $p_n=d_n\circ p$. Then  $p_n \bm{\mathbf{1}}_{A}\nearrow p \bm{\mathbf{1}}_{A}$ and for every $n$, $\mu (p_n \bm{\mathbf{1}}_{A})$ holds. So: 
$$ 
\mu (p \bm{\mathbf{1}}_{A})=\mu (\lim p_n \bm{\mathbf{1}}_{A})=\lim \mu (p_n \bm{\mathbf{1}}_{A})=0
$$
according to the monotone converging theorem, so $\nu$ is absolutely continuous respect to $\mu$


:::

::: {.theorem  name="Radon Nikodym Theorm"}

Suppose that $\mu$ is $\sigma$-finite and $\nu$ is absolutely continuous with repect to $\mu$. Then there exists a positive $\mathcal{E}$-measurable function $p$ s.t. $\nu f=\mu (pf)$ on $E$ for every $f\in \mathcal{E_+}$.  
Moreover, $p$ is unique above, if there is a $q\in \mathcal{E_+}$, then $q=p$ a.e. 

:::

Notice that Randon Nikodym theorem is the converse of the theorem before it.  
The proof of the Randon Nikodym theorem is not able to show here now.


::: {.definition  name="transition kernal"}

Let  $(E,\mathcal{E})$ and $(F,\mathcal{F})$ be measurable spaces. Let $K$ be a mapping from $E\mathcal{\times F}$ into $\overline{\mathbb{R}}_+$. Then, $K$ is called a transition kernal from $(E,\mathcal{E})$ into $(F,\mathcal{F})$ if:
- the mapping $x\mapsto K(x,B)$ is $\mathcal{E}$-measurable for every set $B\in \mathcal{F}$ 
- the mapping $B\mapsto K(x,B)$ is a measure on $(F,\mathcal{F})$ for every $x\in E$

:::

For example, if $\nu$ is a finite measure on $(F,\mathcal{F})$, and $k$ is a positive function on $E\times F$ that is $\mathcal{E\times F}$-measurable, then 
$$ 
K(x,B)=\int_B \nu(dy)k(x,y), \qquad x\in E, B\in \mathcal{F}
$$
when fix $x\in E$, $K(x,B)=\nu(k(x,y)\bm{\mathbf{1}}_{B})=\mu (B)$ for some $\mu$ which is the measure on $(F,\mathcal{F})$.  
when fix $B\in \mathcal{F}$, $K(x,B)=f(x)=$



::: {.theorem  name=""}

Let $K$ be a transition kernal from  $(E,\mathcal{E})$ into $(F,\mathcal{F})$. Then 
$$ 
Kf(x)=\int_F K(x,dy)f(y), \qquad x\in E,
$$
defines a function  $Kf\in \mathcal{E_+}$ for every $f\in \mathcal{F_+}$. 
$$ 
\mu K(B)=\int_E \mu (dx)K(x,B), \qquad B\in \mathcal{F},
$$
defines a measure $\mu K$ on $(F,\mathcal{F})$ for each measure  $\mu$ on $(E,\mathcal{E})$.
and  
$$ 
(\mu K)f=\mu (Kf)=\int_E \mu (dx)\int_F K(x,dy)f(y)
$$
for every measure $\mu$ on $(E,\mathcal{E})$ and function $f$ in $\mathcal{F_+}$.

:::

::: {.proof}



:::

::: {.theorem  name=""}

Let $f\in \mathcal{E\times F}$, then $x\mapsto f(x,y)\in \mathcal{E}$ for each  $y\in F$ and $y\mapsto f(x,y)\in \mathcal{F}$ for each $x\in E$.

:::






















